Updating with motive

theories/Semantics/Cbn.v
@@ -1,4 +1,4 @@
-From Stdlib Require Import List Utf8 Relations Relation_Operators Vectors.Fin.
+From Stdlib Require Import List Utf8 Relations Relation_Operators Vectors.Fin Program.Equality.
 
 From Cyclic.Syntax Require Import StrictPos Term.
 
@@ -46,8 +46,8 @@ Fixpoint shift (d : nat) (c : nat) (t : tm) : tm :=
       tRoll Σ s
         (fun i => shift d c (params i))
         (fun j => shift d c (k j))
-  | tCase Σ scrut br =>
-      tCase Σ (shift d c scrut) (fun s => shift d c (br s))
+  | tCase Σ scrut C br =>
+      tCase Σ (shift d c scrut) C (fun s => shift d c (br s))
   end.
 
 Definition up (σ : nat -> tm) : nat -> tm :=
@@ -67,8 +67,8 @@ Fixpoint subst (σ : nat -> tm) (t : tm) : tm :=
       tRoll Σ s
         (fun i => subst σ (params i))
         (fun j => subst σ (k j))
-  | tCase Σ scrut br =>
-      tCase Σ (subst σ scrut) (fun s => subst σ (br s))
+  | tCase Σ scrut C br =>
+      tCase Σ (subst σ scrut) C (fun s => subst σ (br s))
   end.
 
 Definition subst0 (u : tm) (t : tm) : tm :=
@@ -82,18 +82,36 @@ Inductive step : tm -> tm -> Prop :=
     step (tApp t u) (tApp t' u)
 | step_fix A t :
     step (tFix A t) (subst0 (tFix A t) t)
-| step_case_scrut Σ scrut scrut' br :
+| step_case_scrut Σ scrut scrut' C br :
     step scrut scrut' ->
-    step (tCase Σ scrut br) (tCase Σ scrut' br)
-| step_case_roll Σ s params k br :
-    step (tCase Σ (tRoll Σ s params k) br)
+    step (tCase Σ scrut C br) (tCase Σ scrut' C br)
+| step_case_roll Σ s params k C br :
+    step (tCase Σ (tRoll Σ s params k) C br)
       (apps (br s) (roll_params Σ s params ++ roll_args Σ s k)).
 
-Definition steps : tm -> tm -> Prop := clos_refl_trans tm step.
+Definition steps : tm -> tm -> Prop :=
+  clos_refl_trans tm step.
 
 Inductive value : tm -> Prop :=
 | v_lam A t : value (tLam A t)
 | v_roll Σ s params k : value (tRoll Σ s params k).
+
+(* Neutrals are stuck at the head (no CBN reduction possible). *)
+Inductive neutral : tm -> Prop :=
+| ne_var x : neutral (tVar x)
+| ne_app t u : neutral t -> neutral (tApp t u)
+| ne_case Σ t C br : neutral t -> neutral (tCase Σ t C br).
+
+(* Weak-head normal forms: values or neutrals. *)
+Inductive whnf : tm -> Prop :=
+| whnf_val v : value v -> whnf v
+| whnf_ne t : neutral t -> whnf t.
+
+(* Explicit weak-head evaluation: reduce to a WHNF. *)
+Definition eval_whnf (t w : tm) : Prop :=
+  steps t w ∧ whnf w.
+
+Notation "t ⇓wh w" := (eval_whnf t w) (at level 70).
 
 Definition terminates_to (t v : tm) : Prop :=
   steps t v ∧ value v.
@@ -111,14 +129,175 @@ Proof.
   inversion Hv; subst; inversion Hstep.
 Qed.
 
-Lemma steps_refl (t : tm) : steps t t.
+Lemma neutral_no_step (t t' : tm) :
+  neutral t -> step t t' -> False.
 Proof.
-  apply rt_refl.
+  intro Hn.
+  revert t'.
+  induction Hn as [x|t u Ht IH|Σ t C br Ht IH]; intro t'; intro Hstep.
+  - inversion Hstep.
+  - inversion Hstep; subst.
+    + inversion Ht.
+    + eapply IH; eauto.
+  - inversion Hstep; subst.
+    + eapply IH; eauto.
+    + inversion Ht.
 Qed.
 
-Lemma steps_step (t t' : tm) : step t t' -> steps t t'.
+Lemma whnf_no_step (t t' : tm) :
+  whnf t -> step t t' -> False.
+Proof.
+  intros Hwh Hstep.
+  inversion Hwh; subst.
+  - exact (value_no_step _ _ H Hstep).
+  - exact (neutral_no_step _ _ H Hstep).
+Qed.
+
+(* Determinism of call-by-name stepping. *)
+Lemma step_deterministic (t t1 t2 : tm) :
+  step t t1 -> step t t2 -> t1 = t2.
+Proof.
+  intro H1.
+  revert t2.
+  induction H1 as
+    [A t u
+    | t t' u Htt' IH
+    | A t
+    | Σ scrut scrut' C br Hscrut IH
+    | Σ s params k C br];
+    intro t2; intro H2.
+  - inversion H2; subst; try reflexivity; try discriminate.
+  - inversion H2; subst; try discriminate.
+    + exfalso; inversion Htt'.
+    + f_equal. eapply IH; eauto.
+  - inversion H2; subst; reflexivity.
+  - inversion H2; subst; try discriminate.
+    + (* case-scrut vs case-scrut *)
+      repeat match goal with
+      | H : existT _ _ _ = existT _ _ _ |- _ => dependent destruction H
+      end.
+      pose proof (IH _ H4) as ->.
+      reflexivity.
+    + (* case-scrut vs case-roll is impossible: scrut is a roll, but rolls don't step *)
+      exfalso.
+      eapply value_no_step.
+      * apply v_roll.
+      * exact Hscrut.
+  - inversion H2; subst; try discriminate.
+    + (* case-roll vs case-scrut is impossible: rolls don't step *)
+      exfalso.
+      eapply value_no_step.
+      * apply v_roll.
+      * exact H4.
+    + (* case-roll vs case-roll *)
+      repeat match goal with
+      | H : existT _ _ _ = existT _ _ _ |- _ => dependent destruction H
+      end.
+      reflexivity.
+Qed.
+
+(* A helper for reasoning about multi-step reductions. *)
+Lemma steps_eq_or_step (t u : tm) :
+  steps t u -> t = u ∨ ∃ t', step t t' ∧ steps t' u.
 Proof.
   intro H.
-  apply rt_step.
-  exact H.
+  induction H.
+  - (* rt_step *)
+    right. exists y. split; [exact H|apply rt_refl].
+  - (* rt_refl *)
+    left. reflexivity.
+  - (* rt_trans *)
+    destruct IHclos_refl_trans1 as [->|[t' [Ht' Ht'y]]].
+    + exact IHclos_refl_trans2.
+    + right. exists t'. split.
+      * exact Ht'.
+      * eapply rt_trans; eauto.
+Qed.
+
+Lemma whnf_stuck (w u : tm) :
+  whnf w -> steps w u -> u = w.
+Proof.
+  intros Hwh Hwu.
+  destruct (steps_eq_or_step _ _ Hwu) as [->|[w' [Hwstep _]]].
+  - reflexivity.
+  - exfalso. exact (whnf_no_step _ _ Hwh Hwstep).
+Qed.
+
+Lemma steps_compare (t u v : tm) :
+  steps t u -> steps t v -> steps u v ∨ steps v u.
+Proof.
+  intro Htu.
+  revert v.
+  induction Htu; intro v; intro Htv.
+  - (* rt_step *)
+    destruct (steps_eq_or_step _ _ Htv) as [Heq|[t' [Ht' Ht'v]]].
+    + subst. right. apply rt_step. exact H.
+    + assert (t' = y) by (eapply step_deterministic; eauto).
+      subst t'. left. exact Ht'v.
+  - (* rt_refl *)
+    left. exact Htv.
+  - (* rt_trans *)
+    specialize (IHHtu1 _ Htv) as [Hyv|Hvy].
+    + exact (IHHtu2 _ Hyv).
+    + right. eapply rt_trans; eauto.
+Qed.
+
+Theorem eval_whnf_deterministic (t w1 w2 : tm) :
+  t ⇓wh w1 -> t ⇓wh w2 -> w1 = w2.
+Proof.
+  intros [Ht1 Hw1] [Ht2 Hw2].
+  destruct (steps_compare _ _ _ Ht1 Ht2) as [H12|H21].
+  - symmetry. exact (whnf_stuck _ _ Hw1 H12).
+  - exact (whnf_stuck _ _ Hw2 H21).
+Qed.
+
+(* Big-step weak-head evaluation (inductive), equivalent to ⇓wh. *)
+Inductive eval_whnf_big : tm -> tm -> Prop :=
+| ewhnf_done w : whnf w -> eval_whnf_big w w
+| ewhnf_step t t' w : step t t' -> eval_whnf_big t' w -> eval_whnf_big t w.
+
+Lemma eval_whnf_big_sound (t w : tm) :
+  eval_whnf_big t w -> t ⇓wh w.
+Proof.
+  intro He.
+  induction He as [w Hwh|t t' w Hstep He IH].
+  - split.
+    + apply rt_refl.
+    + exact Hwh.
+  - destruct IH as [Ht'w Hwh].
+    split.
+    + eapply rt_trans.
+      * apply rt_step. exact Hstep.
+      * exact Ht'w.
+    + exact Hwh.
+Qed.
+
+Lemma eval_whnf_big_of_steps (t0 u w : tm) :
+  steps t0 u -> eval_whnf_big u w -> eval_whnf_big t0 w.
+Proof.
+  intro Htu.
+  revert w.
+  dependent induction Htu; intros w He.
+  - (* rt_step *) exact (ewhnf_step _ _ _ H He).
+  - (* rt_refl *) exact He.
+  - (* rt_trans *)
+    apply IHHtu1.
+    apply IHHtu2.
+    exact He.
+Qed.
+
+Lemma eval_whnf_big_complete (t w : tm) :
+  t ⇓wh w -> eval_whnf_big t w.
+Proof.
+  intros [Htw Hwh].
+  apply (eval_whnf_big_of_steps t w w Htw).
+  exact (ewhnf_done w Hwh).
+Qed.
+
+Theorem eval_whnf_big_deterministic (t w1 w2 : tm) :
+  eval_whnf_big t w1 -> eval_whnf_big t w2 -> w1 = w2.
+Proof.
+  intros H1 H2.
+  apply (eval_whnf_deterministic t w1 w2);
+    apply eval_whnf_big_sound; assumption.
 Qed.
